updated M_C and the final proof

demo/DemoB.v
@@ -15,14 +15,16 @@ Definition sum (i: int): int :=
   let sumz: Z := fold_rec Z Z.add 0%Z 0%Z (i.(Int.intval) + 1)%Z in
   Int.repr sumz.
 
-Definition int_int_sg : signature := mksignature (AST.Tint :: nil) (Tret Tint) cc_default.
+Definition int_int_sg : signature := mksignature (AST.Tint :: nil) (Tret AST.Tint) cc_default.
 
-Definition _memoized : ident := 60%positive.
+(** * Implementation of M_A *)
+
+Definition _s : positive := 60%positive.
 Definition lb0: label := 1%positive.
 Definition lb1: label := 2%positive.
 Definition lb2: label := 3%positive.
 
-Definition v_memoized := {|
+Definition v_s := {|
   gvar_info := tt;
   gvar_init := (Init_int32 (Int.zero) :: Init_int32 (Int.zero) :: nil);
   gvar_readonly := false;
@@ -56,7 +58,7 @@ Definition code: list instruction :=
 
      Plabel lb0 ::
      (* .L100: *)
-     Pmovl_rm RAX (Addrmode None None (inr (_memoized, Ptrofs.zero))) ::
+     Pmovl_rm RAX (Addrmode None None (inr (_s, Ptrofs.zero))) ::
      (* movl	memoized(%rip), %eax *)
      Pcmpl_rr RBX RAX ::
      (* cmpl	%eax, %ebx *)
@@ -70,16 +72,16 @@ Definition code: list instruction :=
 
      Pleal RAX (Addrmode (Some RAX) (Some (RBX, 1)) (inl 0)) ::
      (* leal    0(%eax,%ebx,1), %eax *)
-     Pmovl_mr (Addrmode None None (inr (_memoized, Ptrofs.zero))) RBX ::
+     Pmovl_mr (Addrmode None None (inr (_s, Ptrofs.zero))) RBX ::
      (*	movl	%ebx, memoized(%rip) *)
-     Pmovl_mr (Addrmode None None (inr (_memoized, Ptrofs.repr 4))) RAX ::
+     Pmovl_mr (Addrmode None None (inr (_s, Ptrofs.repr 4))) RAX ::
      (*	movl	%eax, (memoized + 4)(%rip) *)
      Pjmp_l lb1 ::
      (* jmp    .L101 *)
 
      Plabel lb2 ::
      (* .L102: *)
-     Pmovl_rm RAX (Addrmode None None (inr (_memoized, Ptrofs.repr 4))) ::
+     Pmovl_rm RAX (Addrmode None None (inr (_s, Ptrofs.repr 4))) ::
      (* movl	(memoized + 4)(%rip), %eax *)
 
      Plabel lb1 ::
@@ -92,18 +94,87 @@ Definition code: list instruction :=
        (* ret *)
      nil.
 
-Definition func_g: function :=
-  mkfunction (int_int_sg) code.
+Definition func_g: Asm.function :=
+  Asm.mkfunction (int_int_sg) code.
 
 Definition global_definitions : list (ident * globdef fundef unit) :=
 ((f_id, Gfun(External (EF_external "f" int_int_sg))) ::
-  (_memoized, Gvar v_memoized) ::
+  (_s, Gvar v_s) ::
   (g_id, Gfun(Internal func_g)) ::
   nil).
 
 Definition public_idents : list ident :=
 (f_id :: g_id :: nil).
 
-Definition prog: program := mkprogram global_definitions public_idents main_id.
+Definition M_A: program := mkprogram global_definitions public_idents main_id.
 
-Definition asm_semantics := Asm.semantics prog.
+Definition asm_semantics := Asm.semantics M_A.
+
+(** * Clight implementation of M_C *)
+Require Import Ctypes Cop Clight Clightrel.
+Require Import Clightdefs.
+
+Local Open Scope Z_scope.
+
+Definition _memoized : ident := 54%positive.
+Definition _t : ident := 56%positive.
+Definition _x : ident := 55%positive.
+Definition _t'1 : ident := 59%positive.
+
+Definition v_memoized := {|
+  gvar_info := (tarray tint MAX);
+  gvar_init := (Init_space (4 * MAX) :: nil);
+  gvar_readonly := false;
+  gvar_volatile := false
+|}.
+
+Definition func_f := {|
+  fn_return := tint;
+  fn_callconv := cc_default;
+  fn_params := ((_x, tint) :: nil);
+  fn_vars := nil;
+  fn_temps := ((_t, tint) :: (_t'1, tint) :: nil);
+  fn_body :=
+(Ssequence
+  (Sifthenelse (Ebinop Oeq (Etempvar _x tint) (Econst_int (Int.repr 0) tint)
+                 tint)
+    (Sreturn (Some (Econst_int (Int.repr 0) tint)))
+    Sskip)
+  (Ssequence
+    (Sset _t
+      (Ederef
+        (Ebinop Oadd (Evar _memoized (tarray tint 1000)) (Etempvar _x tint)
+          (tptr tint)) tint))
+    (Ssequence
+      (Sifthenelse (Ebinop Oeq (Etempvar _t tint)
+                     (Econst_int (Int.repr 0) tint) tint)
+        (Ssequence
+          (Ssequence
+            (Scall (Some _t'1)
+              (Evar g_id (Tfunction (Tcons tint Tnil) tint cc_default))
+              ((Ebinop Osub (Etempvar _x tint) (Econst_int (Int.repr 1) tint)
+                 tint) :: nil))
+            (Sset _t
+              (Ebinop Oadd (Etempvar _t'1 tint) (Etempvar _x tint) tint)))
+          (Sassign
+            (Ederef
+              (Ebinop Oadd (Evar _memoized (tarray tint 1000))
+                (Etempvar _x tint) (tptr tint)) tint) (Etempvar _t tint)))
+        Sskip)
+      (Sreturn (Some (Etempvar _t tint))))))
+|}.
+
+Definition composites : list composite_definition := nil.
+
+Definition global_definitions_c : list (ident * globdef fundef type) :=
+((g_id,
+   Gfun(External (EF_external "g" int_int_sg )
+     (Tcons tint Tnil) tint cc_default)) :: (_memoized, Gvar v_memoized) ::
+ (f_id, Gfun(Internal func_f)) :: nil).
+
+Definition public_idents_c : list ident :=
+(f_id :: g_id :: nil).
+
+Definition M_C : Clight.program :=
+  mkprogram composites global_definitions_c public_idents_c main_id Logic.I.
+
